more defining the language and a bunch of properties

Triposes/Language/Basic.lean
@@ -14,79 +14,12 @@ namespace Language
     /- Fix a tripos -/
     variable {P : 𝒞ᵒᵖ ⥤ HeytAlg} [T : Tripos P]
 
-    -- /- To simplify the definition of `proj`, we use the terminal object of `𝒞` as the default element of `𝒞`. -/
-    -- instance : Inhabited 𝒞 where default := 𝟙_ 𝒞
-
-    -- /-- The product of a list of objects, where we make sure that the product of `[A]` is `A`, rather than `A ⊗ 𝟙_ 𝒞`. -/
-    -- @[reducible]
-    -- def listProd : Lean.AssocList Lean.Name 𝒞 → 𝒞
-    -- | .nil => 𝟙_ 𝒞
-    -- | .cons _ A .nil => A
-    -- | .cons _ A As => A ⊗ listProd As
-
-    -- @[simp]
-    -- def lookup (As : Lean.AssocList Lean.Name 𝒞) (x : Lean.Name) : 𝒞 := (As.find? x).getD (𝟙_ 𝒞)
-
-    -- /-- The k-th projection from a product, or the terminal morphism if the index is invalid -/
-    -- @[reducible]
-    -- def proj (As : Lean.AssocList Lean.Name 𝒞) (x : Lean.Name) : listProd As ⟶ lookup As x :=
-    --   match As  with
-    --   | .nil => fp.toUnit _ -- invalid index
-
-    --   | .cons x' A .nil =>
-    --     if h : x' = x then
-    --       (by
-    --        simp [Lean.AssocList.find?, h]
-    --        exact 𝟙 A)
-    --     else
-    --       (by
-    --        simp [Lean.AssocList.find?, not_beq_of_ne h]
-    --        exact fp.toUnit _)
-
-    --   | .cons x' A (.cons y B Bs) =>
-    --     if h : x' = x then
-    --       (by
-    --       simp [Lean.AssocList.find?, h]
-    --       exact fp.fst _ _
-    --       )
-    --     else
-    --       (by
-    --        simp [Lean.AssocList.find?, not_beq_of_ne h]
-    --        exact fp.snd _ _ ≫ proj (.cons y B Bs) x)
-
-    -- /-- Given an association list of objects `As = [x₀ : A₀, …, xₙ : Aₙ]` we can form expressions that denote
-    --     morphisms `A₀ ⊗ ⋯ ⊗ Aₙ ⟶ B` but are written as if objects are sets. -/
-    -- inductive Expr (As : Lean.AssocList Lean.Name 𝒞) : 𝒞 → Type _ where
-    --   /-- Variable `var x` refers to the `x`-th element of `As`. -/
-    --   | var : ∀ (x : Lean.Name), Expr As (lookup As x)
-    --   /-- The unique element of the terminal object -/
-    --   | tt : Expr As (𝟙_ _)
-    --   /-- Ordered pair -/
-    --   | pair : ∀ {B C}, Expr As B → Expr As C → Expr As (B ⊗ C)
-    --   /-- First projection -/
-    --   | fst : ∀ {B C}, Expr As (B ⊗ C) → Expr As B
-    --   /-- Second projection -/
-    --   | snd : ∀ {B C}, Expr As (B ⊗ C) → Expr As C
-    --   /-- Application of a morphism -/
-    --   | app : ∀ {B C : 𝒞}, (B ⟶ C) → Expr As B → Expr As C
-
-
-    -- /-- Evaluate an expression to the corresponding morphism -/
-    -- @[reducible]
-    -- def Expr.eval (As : Lean.AssocList Lean.Name 𝒞) {B : 𝒞} : Expr As B → (listProd As ⟶ B)
-    --   | .var k => proj As k
-    --   | .tt => fp.toUnit _
-    --   | .pair a b => fp.lift a.eval b.eval
-    --   | .fst a => a.eval ≫ fp.fst _ _
-    --   | .snd a => a.eval ≫ fp.snd _ _
-    --   | .app f a => a.eval ≫ f
-
-
-    /-- `Formula As` denotes a predicate in `P (listProd As)`.
-        It should be easy to add other connectives and quantifiers. -/
-    inductive Formula' : 𝒞 → Type _ where
+    /-- `Formula As` denotes a predicate in `P (listProd As)`. -/
+    inductive Formula' [T : Tripos P] : 𝒞 → Type _ where
+      /-- Injection from underlying structure-/
+    | ι : ∀ {As}, P₀ (P := P) As → Formula' As
       /-- Application of a predicate to an expression -/
-    | app : ∀ {B As}, P₀ (P := P) B → (As ⟶ B) → Formula' As
+    | app : ∀ {B As}, Formula' B → (As ⟶ B) → Formula' As
       /-- The true predicate -/
     | tru : ∀ {As}, Formula' As
       /-- The false predicate -/
@@ -103,7 +36,8 @@ namespace Language
     | any : ∀ {Bs As}, (Bs ⟶ As) → Formula' Bs → Formula' As
 
     def Formula'.eval {As : 𝒞} : Formula' (P := P) As → P₀ (P := P) As
-    | .app ρ f => P₁ f ρ
+    | .ι x => x
+    | .app ρ f => P₁ f (eval ρ)
     | .tru => ⊤
     | .fal => ⊥
     | .conj φ ψ => eval φ ⊓ eval ψ
@@ -116,17 +50,13 @@ namespace Language
 
     def Formula (As : 𝒞) := Quot (Formula_Eq (As := As) (P := P))
 
-    def ι {As : 𝒞} := Quot.mk (Formula_Eq (As := As) (P := P))
+    @[simp]
+    def q {As : 𝒞} := Quot.mk (Formula_Eq (As := As) (P := P))
 
-    def Formula.app {B As : 𝒞} (ρ : P₀ (P := P) B) (f : As ⟶ B) : Formula (P := P) As := Quot.mk Formula_Eq (Formula'.app ρ f)
-    def Formula.tru {As : 𝒞} := ι (P := P) (Formula'.tru (As := As))
-    def Formula.fal {As : 𝒞} := ι (P := P) (Formula'.fal (As := As))
-    -- def Formula.conj {As : 𝒞} (φ ψ : Formula As) := Quot.mk Formula_Eq (Formula'.conj φ ψ)
-    -- def Formula.disj {As : 𝒞} (φ ψ : Formula As) := Quot.mk Formula_Eq (Formula'.disj φ ψ)
-    -- def Formula.impl {As : 𝒞} (φ ψ : Formula As) := Quot.mk Formula_Eq (Formula'.impl φ ψ)
-    -- def Formula.all {Bs As : 𝒞} (f : Bs ⟶ As) (φ : Formula (P := P) Bs) := ι (P := P) (Formula'.all f φ)
-    -- def Formula.any {Bs As : 𝒞} (f : Bs ⟶ As) (φ : Formula (P := P) Bs) := ι (P := P) (Formula'.any f φ)
 
+    def Formula.ι {As : 𝒞} (x : P₀ (P := P) As) : Formula (P := P) As := q (P := P) (.ι x)
+    def Formula.tru {As : 𝒞} : Formula (P := P) As := q (P := P) (.tru (As := As))
+    def Formula.fal {As : 𝒞} : Formula (P := P) As := q (P := P) (.fal (As := As))
 
     syntax "unfold_quotient" : tactic
     syntax "formula_unop_cong" : tactic
@@ -139,30 +69,40 @@ namespace Language
       | `(tactic| formula_unop_cong) =>
         `(tactic| rintro _ _ H; unfold_quotient; rw [H])
 
-    def Formula.conj {As : 𝒞} :=
+    def Formula.app {B As : 𝒞} : Formula (P := P) B → (f : As ⟶ B) → Formula (P := P) As :=
+      Quot.lift (r := Formula_Eq)
+      (fun φ ↦ q (P := P) ∘ Formula'.app (As := As) (B := B) φ)
+      (by
+        rintro _ _ H
+        funext
+        unfold_quotient
+        rw [H]
+      )
+
+    def Formula.conj {As : 𝒞} : Formula (P := P) As → Formula (P := P) As → Formula (P := P) As :=
       Quot.lift₂ (r := Formula_Eq) (s := Formula_Eq)
-      (fun φ ↦ ι (P := P) ∘ (Formula'.conj (As := As) φ))
+      (fun φ ↦ q (P := P) ∘ (Formula'.conj (As := As) φ))
       (by formula_binop_cong)
       (by formula_binop_cong)
 
-    def Formula.disj {As : 𝒞} :=
+    def Formula.disj {As : 𝒞} : Formula (P := P) As → Formula (P := P) As → Formula (P := P) As :=
       Quot.lift₂ (r := Formula_Eq) (s := Formula_Eq)
-      (fun φ ↦ ι (P := P) ∘ (Formula'.disj (As := As) φ))
+      (fun φ ↦ q (P := P) ∘ (Formula'.disj (As := As) φ))
       (by formula_binop_cong)
       (by formula_binop_cong)
 
-    def Formula.impl {As : 𝒞} :=
+    def Formula.impl {As : 𝒞} : Formula (P := P) As → Formula (P := P) As → Formula (P := P) As :=
       Quot.lift₂ (r := Formula_Eq) (s := Formula_Eq)
-      (fun φ ↦ ι (P := P) ∘ (Formula'.impl (As := As) φ))
+      (fun φ ↦ q (P := P) ∘ (Formula'.impl (As := As) φ))
       (by formula_binop_cong)
       (by formula_binop_cong)
 
-    def Formula.all {Bs As : 𝒞} (f : As ⟶ Bs) :=
-      Quot.lift (r := Formula_Eq) (ι (P := P) ∘ Formula'.all f)
+    def Formula.all {Bs As : 𝒞} (f : As ⟶ Bs) : Formula (P := P) As → Formula (P := P) Bs :=
+      Quot.lift (r := Formula_Eq) (q (P := P) ∘ Formula'.all f)
       (by formula_unop_cong)
 
-    def Formula.any {Bs As : 𝒞} (f : As ⟶ Bs) :=
-      Quot.lift (r := Formula_Eq) (ι (P := P) ∘ Formula'.any f)
+    def Formula.any {Bs As : 𝒞} (f : As ⟶ Bs) : Formula (P := P) As → Formula (P := P) Bs :=
+      Quot.lift (r := Formula_Eq) (q (P := P) ∘ Formula'.any f)
       (by formula_unop_cong)
 
     @[reducible]
@@ -172,6 +112,9 @@ namespace Language
           exact H
         )
     def Formula.eval {As : 𝒞} (φ : Formula (P := P) As) : P₀ (P := P) As := Formula.eval' φ
+
+    instance {As : 𝒞} : Coe (P₀ (P := P) As) (Formula (P := P) As) where
+      coe x := .ι x
 
   end Structure
 
@@ -183,6 +126,7 @@ namespace Language
     declare_syntax_cat fpformula
     syntax "⊤" : fpformula
     syntax "⊥" : fpformula
+    syntax ident : fpformula
     syntax:70 fpformula "⊓" fpformula:71 : fpformula
     syntax:60 fpformula "⊔" fpformula:61 : fpformula
     syntax:50 fpformula "⇒" fpformula:51 : fpformula
@@ -209,38 +153,8 @@ namespace Language
         return Array.mk (j :: As.toList)
     | _ => Macro.throwError "invalid context syntax"
 
-    -- macro_rules
-    -- | `($Γ:fpcontext ⊢ₕ ⟪ $f:term | $t:fpterm ⟫) => do
-    --   let t ← `($Γ:fpcontext ⊢ₑ $t)
-    --   `(P₁ $t $f)
-    -- | `($Γ:fpcontext ⊢ₕ $s:fpformula ⊓ $t:fpformula) => do
-    --   let s ← `($Γ:fpcontext ⊢ₕ $s)
-    --   let t ← `($Γ:fpcontext ⊢ₕ $t)
-    --   `($s ⊓ $t)
-    -- | `($Γ:fpcontext ⊢ₕ $s:fpformula ⊔ $t:fpformula) => do
-    --   let s ← `($Γ:fpcontext ⊢ₕ $s)
-    --   let t ← `($Γ:fpcontext ⊢ₕ $t)
-    --   `($s ⊔ $t)
-    -- | `($Γ:fpcontext ⊢ₕ $s:fpformula ⇒ $t:fpformula) => do
-    --   let s ← `($Γ:fpcontext ⊢ₕ $s)
-    --   let t ← `($Γ:fpcontext ⊢ₕ $t)
-    --   `($s ⇨ $t)
-    -- | `($Γ:fpcontext ⊢ₕ $s:fpformula ⇔ $t:fpformula) => do
-    --   let s ← `($Γ:fpcontext ⊢ₕ $s)
-    --   let t ← `($Γ:fpcontext ⊢ₕ $t)
-    --   `($s ⇔ $t)
-    -- | `($_:fpcontext ⊢ₕ ⊤) => `(⊤)
-    -- | `($_:fpcontext ⊢ₕ ⊥) => `(⊥)
-    -- | `($jdgs:typing_judgement,* ⊢ₕ ∀ $y:ident : $Y:term , $t:fpformula) => do
-    --   let t ← `($jdgs:typing_judgement,* , $y:ident : $Y:term ⊢ₕ $t)
-    --   `((Tripos.𝔸 (ChosenFiniteProducts.fst _ _)).map $t)
-    -- | `($jdgs:typing_judgement,* ⊢ₕ ∃ $y:ident : $Y:term , $t:fpformula) => do
-    --   let t ← `($jdgs:typing_judgement,* , $y:ident : $Y:term  ⊢ₕ $t)
-    --   `((Tripos.𝔼 (ChosenFiniteProducts.fst _ _)).map $t)
-    -- | `($Γ:fpcontext ⊢ₕ ($t:fpformula)) => `($Γ:fpcontext ⊢ₕ $t)
-    -- | `($Γ:fpcontext ⊢ $t:fpformula) => `(($Γ:fpcontext ⊢ₕ $t) ≥ ⊤)
-
     macro_rules
+    | `($Γ:fpcontext ⊢ₕ $x:ident) => do `($x)
     | `($Γ:fpcontext ⊢ₕ ⟪ $f:term | $t:fpterm ⟫) => do
       let t ← `($Γ:fpcontext ⊢ₑ $t)
       `(Formula.app $f $t)
@@ -269,8 +183,7 @@ namespace Language
       let t ← `($jdgs:typing_judgement,* , $y:ident : $Y:term  ⊢ₕ $t)
       `(Formula.any (ChosenFiniteProducts.fst _ _) $t)
     | `($Γ:fpcontext ⊢ₕ ($t:fpformula)) => `($Γ:fpcontext ⊢ₕ $t)
-    | `($Γ:fpcontext ⊢ $t:fpformula) => `(⊤ ≤ (Formula.eval (T := by infer_instance) ($Γ:fpcontext ⊢ₕ $t)))
-
+    | `($Γ:fpcontext ⊢ $t:fpformula) => `(Formula.tru = ($Γ:fpcontext ⊢ₕ $t))
 
     namespace Delab
       open PrettyPrinter
