Triposes/Language/Properties.lean
@@ -1,0 +1,206 @@
+import Triposes.Basic
+import Triposes.Language.Basic
+
+open CategoryTheory
+open MonoidalCategory
+
+open Language
+
+section Algebra
+  universe u v
+  variable {𝒞 : Type u} [Category.{v, u} 𝒞]
+  variable {P : 𝒞ᵒᵖ ⥤ HeytAlg} [T : Tripos P]
+
+  variable {As Bs Cs: 𝒞}
+  variable {f g: As ⟶ Bs}
+  variable (α β : Formula (P := P) As)
+  variable {φ ψ : Formula (P := P) As}
+
+  namespace Formula
+
+    def conj_comm : α.conj β = β.conj α := by
+      apply α.ind
+      apply β.ind
+      rintro α β
+      unfold_quotient
+      apply inf_comm
+
+    def disj_comm : α.disj β = β.disj α := by
+      apply α.ind
+      apply β.ind
+      rintro α β
+      unfold_quotient
+      apply sup_comm
+
+  end Formula
+end Algebra
+
+section Map
+  universe u v
+  variable {𝒞 : Type u} [Category.{v, u} 𝒞]
+  variable {P : 𝒞ᵒᵖ ⥤ HeytAlg} [T : Tripos P]
+
+  variable {As Bs Cs: 𝒞}
+  variable {f : As ⟶ Bs} {g : Bs ⟶ Cs}
+  variable {γ : Formula (P := P) Cs}
+
+  -- @[simp]
+  -- theorem map_id {X : 𝒞} {x : P₀ (P := P) X} : Formula.app x (𝟙 X) = x := by
+  --   unfold_quotient
+  --   aesop_cat
+
+  theorem map_comp_app : γ.app (f ≫ g) = (γ.app g).app f := by
+    apply γ.ind
+    rintro γ
+    unfold_quotient
+    aesop_cat
+
+  instance : LE (Formula (P := P) As) := by
+    constructor
+    rintro φ ψ
+    exact φ.eval ≤ ψ.eval
+
+  -- macro_rules
+  --   | `(tactic| unfold_quotient) =>
+  --     `(tactic| apply Quot.sound; unfold Formula_Eq; unfold Formula'.eval; simp)
+  syntax "unfold_quotient_le" : tactic
+  syntax "full_eval" : tactic
+  macro_rules
+    | `(tactic| unfold_quotient_le) =>
+      `(tactic| unfold LE.le; unfold instLEFormula; simp)
+    | `(tactic| full_eval) =>
+      `(tactic| repeat (first | unfold Formula.app | unfold Formula.impl | unfold Formula.conj | unfold Formula.disj | unfold Formula.all | unfold Formula.any))
+
+end Map
+namespace Any
+  universe u v
+  variable {𝒞 : Type u} [Category.{v, u} 𝒞]
+  variable {P : 𝒞ᵒᵖ ⥤ HeytAlg} [T : Tripos P]
+
+  variable {X Y Z As Bs Cs: 𝒞}
+  variable {f : As ⟶ Bs} {g : Bs ⟶ Cs}
+  variable {x : P₀ (P := P) X} {y : P₀ (P := P) Y} {z : P₀ (P := P) Z}
+  variable {φ : Formula (P := P) X} {ψ : Formula (P := P) Y}
+  variable {α : Formula (P := P) As} {β : Formula (P := P) Bs} {γ : Formula (P := P) Cs}
+
+  lemma unit : α ≤ Formula.app (Formula.any f α) f := by
+    unfold_quotient_le
+    apply α.ind
+    rintro α
+    full_eval
+    simp
+    apply (T.𝔼 _).unit
+
+  lemma counit : Formula.any f (Formula.app β f) ≤ β := by
+    apply β.ind
+    intros
+    unfold_quotient_le
+    full_eval
+    simp
+    apply (T.𝔼 _).counit
+
+  lemma id_adj_id : Formula.any (𝟙 _) α = α := by
+    apply α.ind
+    rintro α
+    full_eval
+    simp
+    apply Quot.sound
+    unfold Formula_Eq
+    conv => lhs; unfold Formula'.eval
+    rw [(T.𝔼 _).id_adj_id]
+    simp
+
+  lemma frob_left : Formula.any f (α.conj (β.app f)) = (Formula.any f α).conj β := by
+    apply α.ind
+    apply β.ind
+    rintro α β
+    unfold_quotient
+    conv => lhs; unfold Formula'.eval; enter [2, 2]; unfold Formula'.eval
+    conv => enter [2, 1]; unfold Formula'.eval
+    apply (T.𝔼 _).frob_left
+
+  lemma frob_right : Formula.any f ((β.app f).conj α) = β.conj (Formula.any f α) := by
+    rw [Formula.conj_comm, Formula.conj_comm β]
+    exact frob_left
+
+end Any
+
+namespace All
+  universe u v
+  variable {𝒞 : Type u} [Category.{v, u} 𝒞]
+  variable {P : 𝒞ᵒᵖ ⥤ HeytAlg} [T : Tripos P]
+
+  variable {X Y Z As Bs Cs: 𝒞}
+  variable {f : As ⟶ Bs} {g : Bs ⟶ Cs}
+  variable {x : P₀ (P := P) X} {y : P₀ (P := P) Y} {z : P₀ (P := P) Z}
+  variable {φ : Formula (P := P) X} {ψ : Formula (P := P) Y}
+  variable {α : Formula (P := P) As} {β : Formula (P := P) Bs} {γ : Formula (P := P) Cs}
+
+  lemma unit : β ≤ Formula.all f (Formula.app β f) := by
+    unfold_quotient_le
+    apply β.ind
+    rintro β
+    full_eval
+    simp
+    apply (T.𝔸 _).unit
+
+  lemma counit : Formula.app (Formula.all f α) f ≤ α := by
+    apply α.ind
+    rintro α
+    unfold_quotient_le
+    full_eval
+    simp
+    apply (T.𝔸 _).counit
+
+  lemma id_adj_id : Formula.all (𝟙 _) α = α := by
+    apply α.ind
+    rintro α
+    full_eval
+    simp
+    apply Quot.sound
+    unfold Formula_Eq
+    conv => lhs; unfold Formula'.eval
+    rw [(T.𝔸 _).id_adj_id]
+    simp
+
+  lemma top_eq_top : Formula.all f Formula.tru = Formula.tru (T := T) := by
+    unfold_quotient
+    unfold Formula'.eval
+    apply (T.𝔸 _).top_eq_top
+
+  -- lemma frob_left : Formula.all f (α.disj (β.app f)) = (Formula.all f α).disj β := by
+  --   apply α.ind
+  --   apply β.ind
+  --   rintro α β
+  --   unfold_quotient
+  --   conv => lhs; unfold Formula'.eval; enter [2, 2]; unfold Formula'.eval
+  --   conv => enter [2, 1]; unfold Formula'.eval
+  --   apply (T.𝔸 _).frob_left
+
+  -- lemma frob_right : Formula.all f ((β.app f).disj α) = β.disj (Formula.all f α) := by
+  --   rw [Formula.disj_comm, Formula.disj_comm β]
+  --   exact frob_left
+
+end All
+
+section Adjoints
+  universe u v
+  variable {𝒞 : Type u} [Category.{v, u} 𝒞]
+  variable {P : 𝒞ᵒᵖ ⥤ HeytAlg} [T : Tripos P]
+
+  variable {X Y Z As Bs Cs: 𝒞}
+  variable {f : As ⟶ Bs} {g : Bs ⟶ Cs}
+  variable {x : P₀ (P := P) X} {y : P₀ (P := P) Y} {z : P₀ (P := P) Z}
+  variable {φ : Formula (P := P) X} {ψ : Formula (P := P) Y}
+  variable {α : Formula (P := P) As} {β : Formula (P := P) Bs} {γ : Formula (P := P) Cs}
+
+  lemma frobenius : Formula.all f (α.impl (Formula.app β f)) = (Formula.any f α).impl β := by
+    apply α.ind
+    apply β.ind
+    intros
+    unfold_quotient
+    conv => lhs; unfold Formula'.eval; enter [2, 2]; unfold Formula'.eval
+    conv => enter [2, 1]; unfold Formula'.eval
+    apply T.frobenius
+
+end Adjoints
